Phi_System/PhiSem_Formalization_Tools.thy
@@ -1299,11 +1299,10 @@ proc (nodef) try'':
   argument X
   return YY
   throws EE2
-  \<medium_left_bracket>
-  ;; "__op_try__"
-  ;; F 
-  ;;G
-  ;; \<medium_right_bracket>. .
+  \<medium_left_bracket> "__op_try__"
+    F 
+    G
+  \<medium_right_bracket>. .
 
 proc (nodef) try':
   assumes A: \<open>Union_the_Same_Or_Arbitrary_when_Var Z Y1 Y2\<close>
